library/init/meta/smt/interactive.lean
@@ -20,8 +20,11 @@ repeat close
 meta def step {α : Type} (tac : smt_tactic α) : smt_tactic unit :=
 tac >> solve_goals
 
+meta def istep {α : Type} (line : nat) (col : nat) (tac : smt_tactic α) : smt_tactic unit :=
+λ ss ts, @scope_trace _ line col ((tac >> solve_goals) ss ts)
+
 meta def rstep {α : Type} (line : nat) (col : nat) (tac : smt_tactic α) : smt_tactic unit :=
-λ ss ts, tactic_result.cases_on (@scope_trace _ line col ((tac >> solve_goals) ss ts))
+λ ss ts, tactic_result.cases_on (istep line col tac ss ts)
   (λ ⟨a, new_ss⟩ new_ts, tactic_result.success ((), new_ss) new_ts)
   (λ msg_thunk e ts,
     let msg := msg_thunk () ++ format.line ++ to_fmt "state:" ++ format.line ++ ts^.to_format in
@@ -37,6 +40,9 @@ namespace interactive
 open interactive.types
 
 meta def itactic : Type :=
+smt_tactic unit
+
+meta def irtactic : Type :=
 smt_tactic unit
 
 meta def intros : raw_ident_list → smt_tactic unit
