tests/lean/nested_errors.lean
@@ -1,0 +1,8 @@
+example (a b c : nat) : a = b → c = b → a = c ∧ b = c :=
+begin
+  intros,
+  split,
+  try {intro},    -- Should not report the error here
+  repeat {intro}, -- Should not report the error here
+  abstract { intro,  } -- Should report the error in intro tactic
+end
